

Q6

$$1. m(a+bX) = \frac{1}{N} \sum_{i=1}^N (a+bx_i) = \frac{1}{N} \left( \sum_{i=1}^N a + b \sum_{i=1}^N x_i \right) = \frac{1}{N} (Na) + b \frac{1}{N} \sum_{i=1}^N x_i \\ = a + bm(x)$$

$$2. \text{cov}(X, X) = \frac{1}{N} \sum_{i=1}^N (x_i - m(X))(x_i - m(X)) = \frac{1}{N} \sum_{i=1}^N (x_i - m(X))^2 \\ = s^2$$

$$3. \text{let } Z = a+bY \text{ and } Z_i = a+by_i$$

$$m(Z) = m(a+bY) = a + bm(Y)$$

$$\text{cov}(X, Z) = \frac{1}{N} \sum_{i=1}^N (x_i - m(X))(Z_i - m(Z)) = \frac{1}{N} \sum_{i=1}^N (x_i - m(X))((a+by_i) - (a+bm(Y))) \\ = \frac{1}{N} \sum_{i=1}^N (x_i - m(X)) \cdot b(y_i - m(Y)) = b \cdot \frac{1}{N} \sum_{i=1}^N (x_i - m(X))(y_i - m(Y)) \\ = b \text{cov}(X, Y)$$

$$4. \text{let } U = a+bX, V = a+bY$$

$$U_i - m(U) = b(x_i - m(X)) \text{ and } Z_i - m(Z) = b(y_i - m(Y))$$

$$\text{cov}(U, Z) = \frac{1}{N} \sum_{i=1}^N (U_i - m(U))(Z_i - m(Z)) \\ = \frac{1}{N} \sum_{i=1}^N [b(x_i - m(X))] [b(y_i - m(Y))] \\ = b^2 \left[ \frac{1}{N} \sum_{i=1}^N (x_i - m(X))(y_i - m(Y)) \right] \\ = b^2 \text{cov}(X, Y)$$

5. yes, the transformation  $x \mapsto a+bx$  is strictly increasing  
so it preserves the order of the data

- median is  $Q_{0.5}$  so  $a+b \text{med}(X)$

$$\text{IQR}(a+bX) = (a+bQ_{.75}(X)) - (a+bQ_{.25}(X)) = b(Q_{.75}(X) - Q_{.25}(X)) \\ = b \text{IQR}(X)$$

$$6. \text{let } X = \{0, 2\}$$

$$m(X) = \frac{0+2}{2} = 1 \Rightarrow (m(X))^2 = 1$$

$$X^2 = \{0^2, 2^2\} = \{0, 4\} \Rightarrow m(X^2) = \frac{0+4}{2} = 2$$

$$m(X^2) = 2 \neq 1 = (m(X))^2$$

$$\text{let } X = \{0, 4\}$$

$$m(X) = \frac{0+4}{2} = 2 \Rightarrow \sqrt{m(X)} = \sqrt{2}$$

$$\sqrt{X} = \{\sqrt{0}, \sqrt{4}\} = \{0, 2\} \Rightarrow m(\sqrt{X}) = \frac{0+2}{2} = 1$$

$$m(\sqrt{X}) = 1 \neq \sqrt{2} = \sqrt{m(X)}$$